src/PlutusIR/Semantics/Static/Normalisation/typing_prototype_substA.v
@@ -1,0 +1,406 @@
+Require Import PlutusCert.PlutusIR.
+Require Import PlutusCert.Util.List.
+From PlutusCert Require Import Analysis.BoundVars.
+
+Require Export PlutusCert.PlutusIR.Semantics.Static.Auxiliary.
+Require Export PlutusCert.PlutusIR.Semantics.Static.Context.
+Require Export PlutusCert.PlutusIR.Semantics.Static.Kinding.Kinding.
+Require Export PlutusCert.PlutusIR.Semantics.Static.Normalisation.Normalisation.
+Require Export PlutusCert.PlutusIR.Semantics.Static.TypeSubstitution.
+Require Export PlutusCert.PlutusIR.Semantics.Static.Builtins.Signatures.
+Require Import PlutusCert.PlutusIR.Analysis.BoundVars.
+Require Export PlutusCert.PlutusIR.Analysis.FreeVars.
+From PlutusCert Require Import Dynamic.AnnotationSubstitution.
+
+Require Import micromega.Lia. (* Importing the module for lia tactic *)
+
+From PlutusCert Require Import 
+    Normalisation.Normalisation 
+    Norm_sound_complete
+    PlutusIR 
+    Util.List
+    Static.Util
+    Equality
+    Kinding.Checker
+    Util
+    Dynamic.AnnotationSubstitution
+    SubstituteTCA
+    Size.
+
+From PlutusCert Require Import alpha.util.
+
+Import Coq.Lists.List.
+Import ListNotations.
+Import Coq.Strings.String.
+Local Open Scope string_scope.
+
+Inductive term :=
+  | Var      : name -> term
+  | LamAbs   : binderName -> ty -> term -> term
+  | TyAbs    : binderTyname -> kind -> term -> term.
+
+
+
+Fixpoint substA (X : string) (U : ty) (t : term) {struct t} : term :=
+  match t with
+  | Var y =>
+      Var y
+  | LamAbs bx T t0 =>
+      LamAbs bx (substituteT X U T) (substA X U t0)
+  | TyAbs bX K t0 =>
+      if X =? bX
+        then TyAbs bX K t0
+        else TyAbs bX K (substA X U t0)
+  end.
+
+
+Function size (t : term) : nat :=
+    1 +
+    match t with
+        | Var n           => 0
+        | LamAbs n ty t   => size t
+        | TyAbs n k t     => size t
+    end.
+
+
+Local Open Scope list_scope.
+
+Inductive FreshOver : string -> list string -> Prop :=
+  | FreshOver_nil : forall fr, FreshOver fr []
+  | FreshOver_cons : forall fr x xs, ~ In fr (x :: xs) -> FreshOver fr xs -> FreshOver fr (x :: xs).
+
+Reserved Notation "Delta ',,' Gamma '|-+' t ':' T" (at level 101, t at level 0, T at level 0, no associativity).
+Inductive has_type : list (string * kind) -> list (string * ty) -> term -> ty -> Prop :=
+  | T_Var : forall Γ Δ x T Tn K,
+      lookup x Γ = Coq.Init.Datatypes.Some T ->
+      Δ |-* T : K -> (* Added *)
+      normalise T Tn ->
+      Δ ,, Γ |-+ (Var x) : Tn
+  | T_LamAbs : forall Δ Γ x T1 t T2n T1n,
+      Δ |-* T1 : Kind_Base ->
+      normalise T1 T1n ->
+      Δ ,, (x, T1n) :: Γ |-+ t : T2n ->
+      Δ ,, Γ |-+ (LamAbs x T1 t) : (Ty_Fun T1n T2n)
+  | T_TyAbs : forall Δ Γ X K t Tn Y,
+    (* TODO: Rename in Γ!*)
+      FreshOver Y (map fst Δ) -> (* Do we need more? prolly term/gamma?*)
+      ((Y, K) :: Δ) ,, Γ |-+ (substA X (Ty_Var Y) t) : Tn ->
+      Δ ,, Γ |-+ (TyAbs X K t) : (Ty_Forall Y K Tn)
+
+  where "Δ ',,' Γ '|-+' t ':' T" := (has_type Δ Γ t T).
+
+Definition KB := Kind_Base.
+Definition KB2 := Kind_Base.
+
+Opaque KB.
+Opaque KB2.
+Definition KAB := Kind_Arrow Kind_Base Kind_Base.
+
+Example TyAbsLamAbsEx :
+  nil ,, nil |-+ (TyAbs "X" KB (LamAbs "v" (Ty_Var "X") (Var "v"))  ) : 
+    (Ty_Forall "Y" KB (Ty_Fun (Ty_Var "Y") (Ty_Var "Y"))).
+Proof.
+  constructor.
+  { constructor.
+  (* freshness *) }
+  simpl.
+  constructor.
+  - simpl. constructor. simpl. auto.
+  - constructor.
+  - eapply T_Var. simpl. eauto. constructor. simpl. eauto. constructor.
+Qed.
+
+(* This shows we must not rename in Gamma!*)
+Example TyAbsDouble :
+  nil ,, nil |-+ (TyAbs "X" KB (LamAbs "v" (Ty_Var "X")
+                        (TyAbs "X" KB2 (LamAbs "w" (Ty_Var "X") (Var "v"))))  ) :
+      (Ty_Forall "X" KB (Ty_Fun (Ty_Var "X") 
+                        (Ty_Forall "Y" KB2 (Ty_Fun (Ty_Var "Y") (Ty_Var "X"))))).
+Proof.
+  constructor.
+  { constructor.
+  (* freshness *) }
+  simpl.
+  constructor.
+  - simpl. constructor. simpl. auto.
+  - constructor.
+  - constructor.
+    { constructor. intros Hcontra. inversion Hcontra. simpl in H. inversion H. inversion H. constructor. }
+    simpl.
+    constructor.
+    + constructor. simpl. auto.
+    + constructor.
+    + eapply T_Var with (T := (Ty_Var "X")) (K := KB).
+      * simpl. auto.
+      * constructor. simpl. auto.
+      * constructor.
+Qed.
+      
+
+(*
+type_check ((x, K)::nil) (v, Ty_Var x) (Var v) = Some (Ty_Var x).
+
+type_check ((y, K)::nil) (v, Ty_Var x) (Var v) = Some (Ty_Var y).
+*)
+
+Definition fresh28 (Δ : list (string * kind)) : string := 
+  "a" ++ String.concat EmptyString (map fst Δ).
+
+Lemma fresh28_fresh_over_Δ : forall Δ,
+  FreshOver (fresh28 Δ) (map fst Δ).
+Proof.
+Admitted.
+
+Lemma substA_Var_same_size : forall x y t,
+    size (substA x (Ty_Var y) t) = size t.
+Proof.
+Admitted.
+
+
+From Equations Require Import Equations.
+    
+Equations? type_check (Δ : list (binderTyname * kind)) 
+                     (Γ : list (binderName * ty)) 
+                     (t : term) : option ty 
+  by wf (size t) lt :=
+
+  type_check Δ Γ (Var x) => 
+    match lookup x Γ with
+    | Some T => normaliser_Jacco Δ T
+    | None => None
+    end;
+  type_check Δ Γ (LamAbs x T1 t0) =>
+    match normaliser_Jacco Δ T1 with
+    | Some T1n =>
+        match kind_check Δ T1 with
+        | Some Kind_Base =>
+            match type_check Δ ((x, T1n) :: Γ) t0 with
+            | Some T2 => Some (Ty_Fun T1n T2)
+            | None => None
+            end
+        | _ => None
+        end
+    | None => None
+    end;
+  type_check Δ Γ (TyAbs X K t) =>
+    let Y := fresh28 Δ in
+    (* TODO: Rename in Γ!*)
+    match type_check ((Y, K) :: Δ) Γ (substA X (Ty_Var Y) t) with
+    | Some T => Some (Ty_Forall Y K T)
+    | None => None
+    end.
+
+
+Proof.
+all: intros; simpl; try lia.
+- rewrite substA_Var_same_size. lia.
+Qed.
+
+Inductive AlphaVar : list (string * string) -> string -> string -> Prop :=
+| alpha_var_refl x : AlphaVar [] x x
+| alpha_var_cons z w sigma :
+    AlphaVar ((z, w) :: sigma) z w
+| alpha_var_diff x y z w sigma :
+    x <> z -> 
+    y <> w -> 
+    AlphaVar sigma z w -> 
+    AlphaVar ((x, y) :: sigma) z w.
+
+Inductive Aty : list (string * string) -> ty -> ty -> Prop :=
+| aty_var x y R : 
+    AlphaVar R x y -> 
+    Aty R (Ty_Var x) (Ty_Var y)
+| aty_forall x y A s1 s2 R :
+    Aty ((x, y) :: R) s1 s2 -> 
+    Aty R (Ty_Forall x A s1) (Ty_Forall y A s2).
+
+(* terms are Aterm related if their types are Aty related*)
+Inductive Aterm : list (string * string) -> term -> term -> Prop :=
+| Aterm_var x R : 
+    Aterm R (Var x) (Var x)  (* We are only talking about alpha equivalence at type level*)
+| Aterm_lamabs x T1 T2 t1 t2 R :
+    Aty R T1 T2 -> 
+    Aterm R t1 t2 -> 
+    Aterm R (LamAbs x T1 t1) (LamAbs x T2 t2) (* these x are on term-level, they need not change*)
+| Aterm_tyabs x y K t1 t2 R :
+    Aterm ((x, y) :: R) t1 t2 -> 
+    Aterm R (TyAbs x K t1) (TyAbs y K t2).
+
+(* Contextual alpha equivalence: kinding contexts that match alpha contexts*)
+Inductive CAlpha : list (string * string) -> list (string * PlutusIR.kind) -> list (string * PlutusIR.kind) -> Prop :=
+  | calpha_nil D : CAlpha [] D D 
+  | calpha_cons x y K R Δ Δ' :
+    CAlpha R Δ Δ' ->
+    CAlpha ((x, y)::R) ((x, K)::Δ) ((y, K)::Δ').
+
+(* Currently sequential, do we want that? *)
+Definition renTs (R : list (string * string)) (T : ty) : ty :=
+  msubstT (map (fun p => (fst p, Ty_Var (snd p))) R) T.
+
+(* Contextual alpha equivalence: type contexts that match alpha contexts*)
+
+Inductive CΓAlpha : list (string * string) -> list (string * ty) -> list (string * ty) -> Prop :=
+  | cΓalpha_nil R : CΓAlpha R nil nil
+  | cΓalpha_cons x T R Γ Γ' :
+    CΓAlpha R Γ Γ' ->
+    CΓAlpha R ((x, T)::Γ) ((x, renTs R T)::Γ'). (* parallel or sequential?! *)
+
+Require Import Coq.Program.Equality.
+
+Lemma type_checking_preserves_alpha : forall x y K Δ Δ' Γ Γ' t t' T T' R,
+    Aterm  ((x, y)::R) t t' ->
+    CAlpha ((x, y)::R) ((x, K)::Δ) ((y, K)::Δ') ->
+    Aty    ((x, y)::R) T T' ->
+    CΓAlpha R Γ Γ' ->
+    type_check ((x, K)::Δ) Γ t = Some T ->
+    type_check ((y, K)::Δ') Γ' t' = Some T'.
+Proof.
+  (* Idk where/how yet, but I am pretty confident that we also need to rename types in Γ*)
+  intros.
+  dependent induction H.
+  - autorewrite with type_check. autorewrite with type_check in H3.
+    destruct_match; subst.
+    (* Hmm. If we can find x0 in Γ, then it must already have ben in Δ? So x <> x0?
+      This seems like an implicit invariant on the relation between Γ and Δ.
+    *)
+
+    (* x0 is a term variable, they are not renamed by type-alpha, hence *)
+    assert (
+      (* lookup x0 Γ = Some t -> CΓAlpha R Γ Γ' ->  *)
+      (exists t', (lookup x0 Γ' = Some t') /\ (Aty R t t')))%type.
+    {
+      admit.
+    }
+    destruct H as [t' [Hlookup Ha_t']].
+    rewrite Hlookup.
+  - 
+Admitted.
+
+(* EASY: By construction. *)
+Lemma CAlpha_id : forall Δ,
+    CAlpha (map (fun z => (z, z)) (map fst Δ)) Δ Δ.
+Admitted.
+
+
+(* WRONG: Take Γ = (Ty_Var "x") and t = Var "v" ... *)
+Lemma Delta_rename_preserves_type_checking : forall Δ Γ t T (x y : string) (K : kind),
+    FreshOver y (map fst Δ) -> (* TODO: fresh over type variables in t and T?*)
+    type_check ((x, K)::Δ) Γ t = Some T -> 
+    type_check ((y, K)::Δ) Γ (substA x (Ty_Var y) t) = Some (substituteT x (Ty_Var y) T).
+Proof.
+  intros.
+  remember ((map (fun z => (z, z)) (map fst Δ))) as R.
+  eapply type_checking_preserves_alpha with (R := R); eauto.
+  -
+    (* R are identities, so it is alphaRename on term level
+      I think this only holds if y is fresh over all type variables (bound/fresh) and variables in t.
+      Since substA is non-capture-avoiding, we must not have that y is equal to a binder, then we would 
+      have capture.
+    *)
+    admit.
+  - constructor.
+    rewrite HeqR.
+    apply CAlpha_id.
+  - admit.
+  - 
+    (* R are identities, so it just alphaRename with (x, y)!
+      Suppose T = Ty_Lam y K (Ty_Var x), then of course we cannot rename x to y.
+      Suppose T = Ty_App x y, then of course we cannot rename x to y.
+      Hence y must be fresh over ftv T AND btv T
+
+      Hence, this is exactly the alphaRename lemma (but for Plutus types, instead of ASTLC).
+    *)
+    admit.  
+Admitted.
+
+(* Not right. Take Γ = (Ty_Var "x") and t = Var "v" ... *)
+Lemma Delta_rename_binder : forall Δ Γ t T (x y z : string) (K : kind),
+    (* FreshOver y (map fst Δ) -> TODO: fresh over type variables in t and T? *)
+
+    (* z,y not in Gamma? z, y not in Delta? *)
+    type_check ((y, K)::Δ) Γ (substA x (Ty_Var y) t) = Some T -> 
+    type_check ((z, K)::Δ) Γ (substA x (Ty_Var z) t) = Some (substituteT y (Ty_Var z) T).
+Proof.
+Admitted.
+
+
+
+Require Import Coq.Arith.Wf_nat.
+
+Require Import Coq.Program.Equality.
+
+(* Induction hypothesis strengthened by well founded inductino on size of terms*)
+Theorem type_checking_sound : 
+ forall Δ Γ t T, type_check Δ Γ t = Some T -> (Δ ,, Γ |-+ t : T).
+Proof with (try apply kind_checking_sound; try eapply normaliser_Jacco_sound; eauto).
+    intros.
+    remember (size t) as n.
+    generalize dependent t.
+    generalize dependent T.
+    generalize dependent Δ.
+    generalize dependent Γ.
+    induction n using lt_wf_ind.
+    intros.
+    induction t; intros.
+    - autorewrite with type_check in H0.
+      destruct_match.
+      pose proof (normaliser_Jacco__well_kinded _ _ _ H0) as [K H1].
+      eapply T_Var; eauto.
+      eapply normaliser_Jacco_sound; eauto.
+    - autorewrite with type_check in H0.
+      repeat destruct_match; subst.
+      inversion H0; subst; clear H0.
+      pose proof (normaliser_Jacco__well_kinded _ _ _ Heqo) as [K H1].
+      eapply kind_checking_sound in Heqo0.
+      eapply T_LamAbs; eauto.
+      + apply normaliser_Jacco_sound in Heqo. auto.
+      + eapply H; eauto.
+        simpl. lia.
+    - autorewrite with type_check in H0.
+      simpl in H0.
+      destruct_match.
+      inversion H0; subst. clear H0.
+      constructor.
+      + apply fresh28_fresh_over_Δ.
+      + eapply H; eauto.
+        rewrite substA_Var_same_size. simpl. lia.
+Qed.
+    
+Theorem type_checking_complete : 
+ forall Δ Γ t T, (Δ ,, Γ |-+ t : T) -> exists T', type_check Δ Γ t = Some T' /\ Aty nil T T'.
+Proof with (try apply kind_checking_complete; try eapply normaliser_Jacco_complete; eauto).
+    intros.
+    (* remember (size t) as n.
+    generalize dependent t.
+    generalize dependent T.
+    generalize dependent Δ.
+    generalize dependent Γ.
+    induction n using lt_wf_ind. *)
+    (* intros. *)
+    induction H; intros; simpl.
+    - autorewrite with type_check.
+      rewrite H.
+      exists Tn.
+      split.
+      + eapply normaliser_Jacco_complete; eauto.
+      + (* alpha_refl*)
+        admit.
+    - admit.
+    - destruct IHhas_type as [T' [Heqn Ha]].
+      eexists.
+
+      autorewrite with type_check.
+      simpl.
+      eapply Delta_rename_binder in Heqn.
+      rewrite Heqn.
+      split.
+      eauto.
+      constructor.
+      (* substituteT rename*)
+      admit.
+      apply fresh28_fresh_over_Δ.
+
+Admitted.
+
+
+
